Added support for stateful (ST) effect loops

krmllib/dist/generic/C_Loops.h
@@ -14,9 +14,15 @@
 
 extern void C_Loops_for(uint32_t start, uint32_t finish, void (*f)(uint32_t x0));
 
+extern void C_Loops_for_st(uint32_t start, uint32_t finish, void (*f)(uint32_t x0));
+
 extern void C_Loops_for64(uint64_t start, uint64_t finish, void (*f)(uint64_t x0));
 
+extern void C_Loops_for64_st(uint64_t start, uint64_t finish, void (*f)(uint64_t x0));
+
 extern void C_Loops_reverse_for(uint32_t start, uint32_t finish, void (*f)(uint32_t x0));
+
+extern void C_Loops_reverse_for_st(uint32_t start, uint32_t finish, void (*f)(uint32_t x0));
 
 typedef struct K___uint32_t_bool_s
 {
@@ -29,7 +35,13 @@ extern K___uint32_t_bool
 C_Loops_interruptible_for(uint32_t start, uint32_t finish, bool (*f)(uint32_t x0));
 
 extern K___uint32_t_bool
+C_Loops_interruptible_for_st(uint32_t start, uint32_t finish, bool (*f)(uint32_t x0));
+
+extern K___uint32_t_bool
 C_Loops_interruptible_reverse_for(uint32_t start, uint32_t finish, bool (*f)(uint32_t x0));
+
+extern K___uint32_t_bool
+C_Loops_interruptible_reverse_for_st(uint32_t start, uint32_t finish, bool (*f)(uint32_t x0));
 
 typedef void *C_Loops_repeat_range_body_interp;
 
